theories/logic/sem_types.v
@@ -7,14 +7,15 @@
 
 From iris.proofmode Require Import base tactics.
 From iris.algebra Require Import ofe list.
-From iris.base_logic Require Export lib.iprop.
-From iris.base_logic Require Import upred.
+From iris.base_logic Require Export iprop upred invariants.
 
 (* Hazel Reasoning *)
 From program_logic Require Import weakest_precondition 
-                                  state_reasoning.
+                                  state_reasoning
+                                  protocols.
 
 (* Local imports *)
+From affine_tes.lib Require Import logic.
 From affine_tes.lang Require Import hazel.
 From affine_tes.lang Require Import subst_map.
 From affine_tes.logic Require Import iEff.
@@ -26,7 +27,12 @@ Definition sem_ty_bool {Σ} : sem_ty Σ := (λ v, ∃ b : bool, ⌜ v = #b ⌝)%
 Definition sem_ty_int {Σ} : sem_ty Σ := (λ v, ∃ n : Z, ⌜ v = #n ⌝)%I.
 Definition sem_ty_moved {Σ} : sem_ty Σ := (λ v, True)%I.
 
-(* Reference Type *)
+(* Copyable Reference Type *)
+Definition tyN := nroot .@ "ty".
+Definition sem_ty_ref_cpy `{heapGS Σ} (τ : sem_ty Σ): sem_ty Σ := 
+  (λ v, ∃ l : loc, ⌜ v = #l ⌝ ∗ inv (tyN .@ l) (∃ w, l ↦ w ∗ τ w))%I.
+
+(* Substructural Reference Type *)
 Definition sem_ty_ref `{!heapGS Σ} (τ : sem_ty Σ): sem_ty Σ := 
   (λ v, ∃ l : loc, ⌜ v = #l ⌝ ∗ (∃ w, l ↦ w ∗ τ w))%I.
 
@@ -40,9 +46,9 @@ Definition sem_ty_sum {Σ} (τ κ : sem_ty Σ) : sem_ty Σ :=
 
 (* Affine Arrow type. *)
 Definition sem_ty_aarr `{irisGS eff_lang Σ}
-  (ρ : sem_sig Σ)
   (Γ₁ : env Σ)
   (Γ₂ : env Σ)
+  (ρ : sem_sig Σ)
   (τ : sem_ty Σ)
   (κ : sem_ty Σ) : sem_ty Σ :=
   (λ (v : val),
@@ -53,9 +59,9 @@ Definition sem_ty_aarr `{irisGS eff_lang Σ}
 
 (* Unrestricted Arrow type. *)
 Definition sem_ty_uarr `{irisGS eff_lang Σ} 
-  (ρ : sem_sig Σ)
   (Γ₁ : env Σ)
   (Γ₂ : env Σ)
+  (ρ : sem_sig Σ)
   (τ : sem_ty Σ)
   (κ : sem_ty Σ) : sem_ty Σ :=
   (λ (v : val), □ (
@@ -64,27 +70,11 @@ Definition sem_ty_uarr `{irisGS eff_lang Σ}
       τ w -∗ 
       EWP (v <_ map (subst_map vs ∘ Var) (env_dom Γ₁) _> w) <| ρ |> {{ u, κ u ∗ ⟦ Γ₂ ⟧ vs }}))%I.
 
-Definition discrete_fun_app {Σ} A (P Q : A -d> iPropO Σ) x n :
-  P ≡{n}≡ Q → (P x) ≡{n}≡ (Q x).
-Proof. intros H. f_equiv. Qed.
-
-Definition discrete_fun_app3 {Σ} A B C (P Q : A -d> B -d> C -d> iPropO Σ) x1 x2 x3 n :
-  P ≡{n}≡ Q → (P x1 x2 x3) ≡{n}≡ (Q x1 x2 x3).
-Proof. intros H. apply discrete_fun_app. f_equiv. Qed.
-
-Definition discrete_fun_app4 {Σ} A B C D (P Q : A -d> B -d> C -d> D -d> iPropO Σ) x1 x2 x3 x4 n :
-  P ≡{n}≡ Q → (P x1 x2 x3 x4) ≡{n}≡ (Q x1 x2 x3 x4).
-Proof. intros H. apply discrete_fun_app3. f_equiv. Qed.
-
-Definition discrete_fun_app5 {Σ} A B C D E (P Q : A -d> B -d> C -d> D -d> E -d> iPropO Σ) x1 x2 x3 x4 x5 n :
-  P ≡{n}≡ Q → (P x1 x2 x3 x4 x5) ≡{n}≡ (Q x1 x2 x3 x4 x5).
-Proof. intros H. apply discrete_fun_app4. f_equiv. Qed.
-
 (* Sequentially Unrestricted Arrow type. *)
 Definition sem_ty_suarr_pre `{irisGS eff_lang Σ} 
-  (ρ : sem_sig Σ)
   (Γ₁ : env Σ)
   (Γ₂ : env Σ)
+  (ρ : sem_sig Σ)
   (τ : sem_ty Σ)
   (κ : sem_ty Σ) 
   (rec : sem_ty Σ) : sem_ty Σ :=
@@ -95,7 +85,7 @@ Definition sem_ty_suarr_pre `{irisGS eff_lang Σ}
 
 Global Instance sem_ty_suarr_pre_contractive `{irisGS eff_lang Σ} 
   (ρ : sem_sig Σ) (Γ₁ Γ₂ : env Σ) (τ κ : sem_ty Σ) :
-  Contractive (sem_ty_suarr_pre ρ Γ₁ Γ₂ τ κ).
+  Contractive (sem_ty_suarr_pre Γ₁ Γ₂ ρ τ κ).
 Proof. 
   intros ????. unfold sem_ty_suarr_pre. intros ?.
   do 2 (rewrite bi.forall_ne; first done; intros ?). f_equiv.
@@ -105,40 +95,40 @@ Proof.
               iEff_bottom (λ u : val, (κ u ∗ ⟦ Γ₂ ⟧ a0 ∗ z x0)%I) ≡{n}≡ 
             ewp_pre (fixpoint ewp_pre) ⊤ (app_mult x0 (map (subst_map a0 ∘ Var) (env_dom Γ₁)) a) ρ
               iEff_bottom (λ u : val, (κ u ∗ ⟦ Γ₂ ⟧ a0 ∗ z x0)%I)).
-  { intros ?. apply discrete_fun_app5. by rewrite  -fixpoint_unfold. }
+  { intros ?. apply non_dep_fun_dist5. by rewrite  -fixpoint_unfold. }
   rewrite (Hunfold x) (Hunfold y). clear Hunfold. rewrite /ewp_pre.
   destruct (to_val) eqn:Hval; first done. 
   destruct (to_eff) eqn:Heff; first done. rewrite -/ewp_pre. simpl.
   do 21 (f_contractive || f_equiv).
   induction num_laters_per_step as [|k IHk]; simpl; last (by rewrite IHk).
   do 2 f_equiv. rewrite -/ewp_def.
-  do 2 f_equiv. intros ?. do 2 f_equiv. by apply sem_ty_dist.
+  do 2 f_equiv. intros ?. do 2 f_equiv. by apply non_dep_fun_dist.
 Qed.
 
 Definition sem_ty_suarr `{irisGS eff_lang Σ}
-  (ρ : sem_sig Σ)
   (Γ₁ Γ₂ : env Σ)
+  (ρ : sem_sig Σ)
   (τ : sem_ty Σ)
-  (κ : sem_ty Σ) : sem_ty Σ := fixpoint (sem_ty_suarr_pre ρ Γ₁ Γ₂ τ κ).
+  (κ : sem_ty Σ) : sem_ty Σ := fixpoint (sem_ty_suarr_pre Γ₁ Γ₂ ρ τ κ).
 
 Lemma sem_ty_suarr_unfold `{irisGS eff_lang Σ}
-  (ρ : sem_sig Σ)
   (Γ₁ Γ₂ : env Σ)
+  (ρ : sem_sig Σ)
   (τ : sem_ty Σ)
   (κ : sem_ty Σ) 
   (v : val) :
-  (sem_ty_suarr ρ Γ₁ Γ₂ τ κ)%V v ⊣⊢
+  (sem_ty_suarr Γ₁ Γ₂ ρ τ κ)%V v ⊣⊢
     (∀ (w : val) (vs : gmap string val),
       ⟦ Γ₁ ⟧ vs -∗ 
       τ w -∗ 
       EWP (v <_ map (subst_map vs ∘ Var) (env_dom Γ₁) _>  w) <| ρ |> {{ u, κ u ∗ 
                                                                            ⟦ Γ₂ ⟧ vs ∗ 
-                                                                           sem_ty_suarr ρ Γ₁ Γ₂ τ κ v }})%I.
+                                                                           sem_ty_suarr Γ₁ Γ₂ ρ τ κ v }})%I.
 Proof.
   unfold sem_ty_suarr. 
-  set suarr := sem_ty_suarr_pre ρ Γ₁ Γ₂ τ κ.
+  set suarr := sem_ty_suarr_pre Γ₁ Γ₂ ρ τ κ.
   assert (Hfix : fixpoint suarr v ≡ suarr (fixpoint suarr) v).
-  { iApply sem_ty_equiv. apply fixpoint_unfold. }
+  { iApply non_dep_fun_equiv. apply fixpoint_unfold. }
   etrans; [apply Hfix|].
   by rewrite /sem_ty_suarr_pre.
 Qed.
@@ -195,7 +185,7 @@ Proof.
   because it is a function.
   As a result we fistly apply sem_ty_equiv lemma *)
   assert (fixpoint (sem_ty_rec_pre C) v ≡ sem_ty_rec_pre C (fixpoint (sem_ty_rec_pre C)) v).
-  { apply sem_ty_equiv. apply fixpoint_unfold. }
+  { apply non_dep_fun_equiv. apply fixpoint_unfold. }
   rewrite H. iSplit.
   - iIntros "(%rec' & #Hrec & HC) !>".
     set Ψ := λ τ, C τ v.
@@ -203,7 +193,7 @@ Proof.
     assert (Ψ (sem_ty_rec C) = C (sem_ty_rec C) v) by done.
     rewrite <- H0. rewrite <- H1.
     iApply (internal_eq_rewrite rec' (sem_ty_rec C)).
-    + intros n τ τ' Hττ'. unfold Ψ. apply sem_ty_dist. 
+    + intros n τ τ' Hττ'. unfold Ψ. apply non_dep_fun_dist.
       by apply NonExpansive0.
     + by iApply internal_eq_sym.
     + iApply "HC".
@@ -211,10 +201,10 @@ Proof.
     by iFrame. 
 Qed.
 
-(* Empty Effect Sig. *)
+(* Empty Effect Signature *)
 Definition sem_sig_nil {Σ} : sem_sig Σ := iEff_bottom.
 
-(* Effect Sig. *)
+(* Effect Signature *)
 Definition sem_sig_eff {Σ} (τ κ : sem_ty Σ) : (sem_sig Σ) :=
   (>> (a : val) >> ! a {{ τ a }}; 
    << (b : val) << ? b {{ κ b }} @OS).
@@ -229,6 +219,108 @@ Lemma sem_sig_eff_eq {Σ} τ κ v Φ :
     (∃ a, ⌜ a = v ⌝ ∗ τ a ∗ (∀ b, κ b -∗ Φ b))%I.
 Proof. by rewrite /sem_sig_eff (iEff_tele_eq' [tele _] [tele _]). Qed.
 
+(* Recursive Effect Signature *)
+
+(* Effect Signature *)
+Definition sem_sig_eff_rec_pre {Σ} (τ κ : sem_sig Σ -d> sem_ty Σ) (rec : sem_sig Σ) : (sem_sig Σ) :=
+  (>> (a : val) >> ! a {{ ▷ (∃ rec', rec ≡ rec' ∧ τ rec' a) }}; 
+   << (b : val) << ? b {{ ▷ (∃ rec', rec ≡ rec' ∧ κ rec' b) }} @OS).
+
+Global Instance sem_sig_eff_rec_pre_contractive {Σ} (τ κ : sem_sig Σ -d> sem_ty Σ) :
+  Contractive (sem_sig_eff_rec_pre τ κ).
+Proof.
+  intros ?????. 
+  rewrite /sem_sig_eff_rec_pre iEffPre_exist_eq iEffPost_exist_eq /=.
+  intros ?. simpl. do 3 f_equiv. rewrite iEffPre_base_eq /=.
+  intros ?. simpl. do 2 f_equiv.
+  { f_contractive. simpl in H. by do 4 f_equiv. }
+  f_equiv. intros ?. rewrite /iEffPost_exist_def. do 3 f_equiv.
+  rewrite iEffPost_base_eq /iEffPost_base_def. f_equiv. f_contractive.
+  simpl in H. by do 4 f_equiv.
+Qed.
+
+Definition sem_sig_eff_rec {Σ} (τ κ : sem_sig Σ -d> sem_ty Σ) : sem_sig Σ :=
+  fixpoint (sem_sig_eff_rec_pre τ κ).
+
+Lemma sem_sig_eff_rec_unfold {Σ} (τ κ : sem_sig Σ -d> sem_ty Σ) `{ NonExpansive τ, NonExpansive κ } :
+  (sem_sig_eff_rec τ κ) ≡ 
+    (>> (a : val) >> ! a {{ ▷ (τ (sem_sig_eff_rec τ κ) a) }}; 
+     << (b : val) << ? b {{ ▷ (κ (sem_sig_eff_rec τ κ) b) }} @OS)%ieff .
+Proof.
+  rewrite {1} /sem_sig_eff_rec fixpoint_unfold {1} /sem_sig_eff_rec_pre.
+  do 4 f_equiv. 
+  - iSplit. 
+    + iIntros "[% [#Hfix Hτ]]". 
+      set Ψ := λ ρ, τ ρ a.
+      replace (τ rec' a) with (Ψ rec') by done.
+      replace (τ (sem_sig_eff_rec τ κ) a) with (Ψ (sem_sig_eff_rec τ κ)) by done.
+      unfold sem_sig_eff_rec.
+      iApply (internal_eq_rewrite rec' (sem_sig_eff_rec τ κ)).
+      { intros ????. unfold Ψ. apply non_dep_fun_dist. by rewrite H. }
+      { by iApply internal_eq_sym. }
+      iApply "Hτ".
+    + iIntros "Hτ //=". iExists (sem_sig_eff_rec τ κ).
+      by iFrame. 
+  - intros ?. rewrite iEffPost_base_eq /iEffPost_base_def.
+    intros ?. do 2 f_equiv. iSplit.
+    + iIntros "[% [#Hfix Hκ]]". 
+      set Ψ := λ ρ, κ ρ a0.
+      replace (κ rec' a0) with (Ψ rec') by done.
+      replace (κ (sem_sig_eff_rec τ κ) a0) with (Ψ (sem_sig_eff_rec τ κ)) by done.
+      unfold sem_sig_eff_rec.
+      iApply (internal_eq_rewrite rec' (sem_sig_eff_rec τ κ)).
+      { intros ????. unfold Ψ. apply non_dep_fun_dist. by rewrite H. }
+      { by iApply internal_eq_sym. }
+      iApply "Hκ".
+    + iIntros "Hτ //=". iExists (sem_sig_eff_rec τ κ).
+      by iFrame. 
+Qed.
+
+Lemma sem_sig_eff_rec_unfold' {Σ} (τ κ : sem_sig Σ -d> sem_ty Σ) `{ NonExpansive τ, NonExpansive κ } v Φ:
+  iEff_car (sem_sig_eff_rec τ κ) v Φ ⊣⊢
+    iEff_car (>> (a : val) >> ! a {{ ▷ (τ (sem_sig_eff_rec τ κ) a) }}; 
+     << (b : val) << ? b {{ ▷ (κ (sem_sig_eff_rec τ κ) b) }} @OS)%ieff v Φ.
+Proof.
+  assert (Hequiv :
+  iEff_car (sem_sig_eff_rec τ κ) v Φ ⊣⊢
+    iEff_car (>> (a : val) >> ! a {{ ▷ (τ (sem_sig_eff_rec τ κ) a) }}; 
+     << (b : val) << ? b {{ ▷ (κ (sem_sig_eff_rec τ κ) b) }} @OS)%ieff v Φ).
+  { f_equiv. apply non_dep_fun_equiv. by apply sem_sig_eff_rec_unfold. }
+  by rewrite Hequiv.
+Qed.
+
+Lemma sem_sig_eff_rec_eq {Σ} τ κ v Φ `{ NonExpansive τ, NonExpansive κ }:
+  iEff_car (sem_sig_eff_rec (Σ:=Σ) τ κ) v Φ ⊣⊢
+    (∃ a, ⌜ a = v ⌝ ∗ (▷ τ (sem_sig_eff_rec τ κ) a) ∗ 
+          (∀ b, (▷ κ (sem_sig_eff_rec τ κ) b) -∗ Φ b))%I.
+Proof. 
+  etrans; [by apply sem_sig_eff_rec_unfold'|]. 
+  by rewrite (iEff_tele_eq' [tele _] [tele _]) /=. 
+Qed.
+
+(* The sem_sig_eff_rec is monotonic. *)
+Global Instance sem_sig_eff_rec_mono_prot {Σ} τ κ `{ NonExpansive τ, NonExpansive κ }:
+  MonoProt (@sem_sig_eff_rec Σ τ κ).
+Proof.
+  constructor. iIntros (???) "HΦ'".
+  rewrite !sem_sig_eff_rec_eq.
+  iIntros "(% & -> & Hτ & HκΦ)".
+  iExists v. iSplitR; first done. iFrame.
+  iIntros (b) "Hκ". iApply "HΦ'". by iApply "HκΦ".
+Qed.
+
+Lemma upcl_sem_sig_rec_eff {Σ} τ κ v Φ `{ NonExpansive τ, NonExpansive κ}:
+  iEff_car (upcl OS (sem_sig_eff_rec (Σ:=Σ) τ κ)) v Φ ⊣⊢
+    (∃ a, ⌜ a = v ⌝ ∗ (▷ τ (sem_sig_eff_rec τ κ) a) ∗ 
+          (∀ b, (▷ κ (sem_sig_eff_rec τ κ) b) -∗ Φ b))%I.
+Proof.
+  assert (Hequiv:
+    iEff_car (upcl OS (sem_sig_eff_rec τ κ)) v Φ ≡
+    iEff_car (sem_sig_eff_rec τ κ) v Φ).
+  { f_equiv. apply non_dep_fun_equiv. by rewrite upcl_id. }
+  rewrite Hequiv. by apply sem_sig_eff_rec_eq.
+Qed.
+
 (* Notations. *)
 Notation "()" := sem_ty_unit : sem_ty_scope.
 Notation "'𝔹'" := (sem_ty_bool) : sem_ty_scope.
@@ -241,6 +333,9 @@ Infix "+" := (sem_ty_sum) : sem_ty_scope.
 Notation "'Ref' τ" := (sem_ty_ref τ%T) 
   (at level 50) : sem_ty_scope.
 
+Notation "'Ref*' τ" := (sem_ty_ref_cpy τ%T) 
+  (at level 50) : sem_ty_scope.
+
 Notation "'∀T:' α , { ρ } ,  C " := (sem_ty_forall ρ (λ α, C%T)) 
   (at level 180) : sem_ty_scope.
 
@@ -250,37 +345,39 @@ Notation "'∀S:' θ , C " := (sem_ty_sig_forall (λ θ, C%T))
 Notation "'∃:' α , C " := (sem_ty_exists (λ α, C%T)) 
   (at level 180) : sem_ty_scope.
 
-Notation "'μ:' α , C " := (sem_ty_rec (λ α, C%T)) 
+Notation "'μT:' α , C " := (sem_ty_rec (λ α, C%T))
   (at level 180) : sem_ty_scope.
 
 Notation "⟨⟩" := sem_sig_nil : sem_sig_scope.
-Notation "τ ⇒ κ" := (sem_sig_eff τ%T κ%T) 
-  (at level 100, κ at level 200) : sem_sig_scope.
+(* Notation "τ ⇒ κ" := (sem_sig_eff τ%T κ%T) *)
+(*   (at level 100, κ at level 200) : sem_sig_scope. *)
+Notation "'μS:' α , τ ⇒ κ" := (sem_sig_eff_rec (λ α, τ%T) (λ α, κ%T))
+  (at level 100, τ, κ at level 200) : sem_sig_scope.
 
-Notation "τ '-{' ρ ; Γ₁ ; Γ₂ '}-∘' κ" := (sem_ty_aarr ρ%R Γ₁ Γ₂ τ%T κ%T)
+Notation "τ '-{' ρ ; Γ₁ ; Γ₂ '}-∘' κ" := (sem_ty_aarr Γ₁ Γ₂ ρ%R τ%T κ%T)
   (at level 100, ρ, κ at level 200) : sem_ty_scope.
-Notation "τ '-{' ρ '}-∘' κ" := (sem_ty_aarr ρ%R [] [] τ%T κ%T)
+Notation "τ '-{' ρ '}-∘' κ" := (sem_ty_aarr [] [] ρ%R τ%T κ%T)
   (at level 100, ρ, κ at level 200) : sem_ty_scope.
-Notation "τ ⊸ κ" := (sem_ty_aarr sem_sig_nil [] [] τ%T κ%T)
+Notation "τ ⊸ κ" := (sem_ty_aarr [] [] sem_sig_nil τ%T κ%T)
   (at level 99, κ at level 200) : sem_ty_scope.
 
-Notation "τ '-{' ρ ; Γ₁ ; Γ₂ '}->' κ" := (sem_ty_uarr ρ%R Γ₁ Γ₂ τ%T κ%T)
+Notation "τ '-{' ρ ; Γ₁ ; Γ₂ '}->' κ" := (sem_ty_uarr Γ₁ Γ₂ ρ%R τ%T κ%T)
   (at level 100, ρ, κ at level 200) : sem_ty_scope.
-Notation "τ '-{' ρ '}->' κ" := (sem_ty_uarr ρ%R [] [] τ%T κ%T)
+Notation "τ '-{' ρ '}->' κ" := (sem_ty_uarr [] [] ρ%R τ%T κ%T)
   (at level 100, ρ, κ at level 200) : sem_ty_scope.
-Notation "τ → κ" := (sem_ty_uarr sem_sig_nil [] [] τ%T κ%T)
+Notation "τ → κ" := (sem_ty_uarr [] [] sem_sig_nil τ%T κ%T)
   (at level 99, κ at level 200) : sem_ty_scope.
 
-Notation "τ '>-{' ρ ; Γ₁ ; Γ₂ '}-∘' κ" := (sem_ty_suarr ρ%R Γ₁ Γ₂ τ%T κ%T)
+Notation "τ '>-{' ρ ; Γ₁ ; Γ₂ '}-∘' κ" := (sem_ty_suarr Γ₁ Γ₂ ρ%R τ%T κ%T)
   (at level 100, ρ, Γ₁, Γ₂, κ at level 200) : sem_ty_scope.
-Notation "τ '>-{' ρ '}-∘' κ" := (sem_ty_suarr ρ%R [] [] τ%T κ%T)
+Notation "τ '>-{' ρ '}-∘' κ" := (sem_ty_suarr [] [] ρ%R τ%T κ%T)
   (at level 100, ρ, κ at level 200) : sem_ty_scope.
-Notation "τ >-∘ κ" := (sem_ty_suarr sem_sig_nil [] [] τ%T κ%T)
+Notation "τ >-∘ κ" := (sem_ty_suarr [] [] sem_sig_nil τ%T κ%T)
   (at level 99, κ at level 200) : sem_ty_scope.
 
 (* Derived Types *)
 
-Definition ListF {Σ} (τ : sem_ty Σ) := λ α, (() + (τ × α))%T.
+Definition ListF {Σ} (τ : sem_ty Σ) := (λ α, () + (τ × α))%T.
 
 (* List type. *)
 Definition sem_ty_list {Σ} (τ : sem_ty Σ) : sem_ty Σ := 
@@ -299,35 +396,40 @@ Notation "'Option' τ" := (sem_ty_option τ%T)
 Section types_properties.
   Context `{heapGS Σ}.
 
-  Ltac solve_non_expansive2 :=
+  Ltac solve_non_expansive :=
     repeat intros ?;
     unfold sem_ty_unit, sem_ty_int, sem_ty_bool,
            sem_ty_prod, sem_ty_sum, sem_ty_aarr,
-           sem_ty_uarr, sem_ty_suarr, sem_ty_ref, sem_ty_rec,
-           sem_ty_list, sem_ty_forall, sem_ty_exists;
-    repeat (f_equiv || done || intros ? || by apply sem_ty_dist).
+           sem_ty_uarr, sem_ty_suarr, sem_ty_ref, sem_ty_ref_cpy,
+           sem_ty_rec, sem_ty_list, sem_ty_forall, sem_ty_exists;
+    repeat (f_equiv || done || intros ? || by apply non_dep_fun_dist).
 
   Global Instance sem_ty_prod_ne : NonExpansive2 (@sem_ty_prod Σ).
-  Proof. solve_non_expansive2. Qed.
+  Proof. solve_non_expansive. Qed.
 
   Global Instance sem_ty_sum_ne : NonExpansive2 (@sem_ty_sum Σ).
-  Proof. solve_non_expansive2. Qed.
+  Proof. solve_non_expansive. Qed.
 
-  Global Instance sem_ty_aarr_ne ρ Γ₁ Γ₂: NonExpansive2 (sem_ty_aarr ρ Γ₁ Γ₂).
-  Proof. solve_non_expansive2. Qed.
+  Global Instance sem_ty_aarr_ne Γ₁ Γ₂: NonExpansive3 (sem_ty_aarr Γ₁ Γ₂).
+  Proof. solve_non_expansive. Qed.
 
-  Global Instance sem_ty_uarr_ne ρ Γ₁ Γ₂ : NonExpansive2 (sem_ty_uarr ρ Γ₁ Γ₂).
-  Proof. solve_non_expansive2. Qed.
+  Global Instance sem_ty_uarr_ne Γ₁ Γ₂ : NonExpansive3 (sem_ty_uarr Γ₁ Γ₂).
+  Proof. solve_non_expansive. Qed.
 
-  Global Instance sem_ty_suarr_ne ρ Γ₁ Γ₂ : NonExpansive2 (sem_ty_suarr ρ Γ₁ Γ₂).
+  Global Instance sem_ty_suarr_ne Γ₁ Γ₂ : NonExpansive3 (sem_ty_suarr Γ₁ Γ₂).
   Proof. 
-    intros ????????. rewrite /sem_ty_suarr. apply sem_ty_dist. apply fixpoint_ne.
-    intros ?. rewrite /sem_ty_suarr_pre. intros ?. repeat f_equiv; [by apply sem_ty_dist|].
-    intros ?. f_equiv. by apply sem_ty_dist.
+    intros ??????????. rewrite /sem_ty_suarr. 
+   apply fixpoint_ne.
+    intros ?. rewrite /sem_ty_suarr_pre. intros ?. 
+    repeat f_equiv; [by apply non_dep_fun_dist|done|].
+    intros ?. f_equiv. by apply non_dep_fun_dist.
   Qed.
 
   Global Instance sem_ty_ref_ne : NonExpansive2 (@sem_ty_ref Σ _).
-  Proof. solve_non_expansive2. Qed.
+  Proof. solve_non_expansive. Qed.
+
+  Global Instance sem_ty_ref_cpy_ne : NonExpansive2 (@sem_ty_ref_cpy Σ _).
+  Proof. solve_non_expansive. Qed.
 
   Global Instance sem_ty_forall_ne n ρ :
     Proper (pointwise_relation _ (dist n) ==> dist n) (sem_ty_forall ρ).
@@ -336,40 +438,43 @@ Section types_properties.
   Global Instance sem_ty_exist_ne n :
     Proper (pointwise_relation _ (dist n) ==> dist n) sem_ty_exists.
   Proof. intros ????. unfold sem_ty_exists; repeat f_equiv. 
-         unfold pointwise_relation in H. by apply sem_ty_dist. Qed.
+         unfold pointwise_relation in H. by apply non_dep_fun_dist. Qed.
 
   Global Instance sem_ty_rec_ne n :
     Proper (pointwise_relation _ (dist n) ==> dist n) (@sem_ty_rec Σ).
   Proof.
     intros C1 C2 HA. unfold sem_ty_rec. apply fixpoint_ne.
     intros ??. unfold sem_ty_rec_pre. do 4 f_equiv. 
-    by apply sem_ty_dist.
+    by apply non_dep_fun_dist.
   Qed.
 
   Global Instance sem_ty_listF_ne τ : NonExpansive (@ListF Σ τ).
   Proof. intros ????. unfold ListF; by repeat f_equiv. Qed.
 
   Global Instance sem_ty_prod_proper : Proper ((≡) ==> (≡) ==> (≡)) (@sem_ty_prod Σ).
-  Proof. solve_non_expansive2. Qed.
+  Proof. solve_non_expansive. Qed.
 
   Global Instance sem_ty_sum_proper : Proper ((≡) ==> (≡) ==> (≡)) (@sem_ty_sum Σ).
-  Proof. solve_non_expansive2. Qed.
+  Proof. solve_non_expansive. Qed.
 
-  Global Instance sem_ty_aarr_proper ρ Γ₁ Γ₂ : Proper ((≡) ==> (≡) ==> (≡)) (sem_ty_aarr ρ Γ₁ Γ₂).
-  Proof. solve_non_expansive2. Qed.
+  Global Instance sem_ty_aarr_proper Γ₁ Γ₂ : Proper ((≡) ==> (≡) ==> (≡) ==> (≡)) (sem_ty_aarr Γ₁ Γ₂).
+  Proof. solve_non_expansive. Qed.
 
-  Global Instance sem_ty_suarr_proper ρ Γ₁ Γ₂ : Proper ((≡) ==> (≡) ==> (≡)) (sem_ty_suarr ρ Γ₁ Γ₂).
+  Global Instance sem_ty_uarr_proper Γ₁ Γ₂ : Proper ((≡) ==> (≡) ==> (≡) ==> (≡)) (sem_ty_uarr Γ₁ Γ₂).
+  Proof. solve_non_expansive. Qed.
+
+  Global Instance sem_ty_suarr_proper Γ₁ Γ₂ : Proper ((≡) ==> (≡) ==> (≡) ==> (≡)) (sem_ty_suarr Γ₁ Γ₂).
   Proof. 
-    intros ??????. apply equiv_dist=>n.
-    apply sem_ty_suarr_ne=> A; [by apply equiv_dist|].
-    apply sem_ty_dist. by apply equiv_dist. 
+    intros ?????????. apply equiv_dist=>n.
+    apply sem_ty_suarr_ne=> A; [by apply equiv_dist| |];
+    apply non_dep_fun_dist; by apply equiv_dist. 
   Qed.
-
-  Global Instance sem_ty_uarr_proper ρ Γ₁ Γ₂ : Proper ((≡) ==> (≡) ==> (≡)) (sem_ty_uarr ρ Γ₁ Γ₂).
-  Proof. solve_non_expansive2. Qed.
 
   Global Instance sem_ty_ref_proper : Proper ((≡) ==> (≡)) (@sem_ty_ref Σ _).
   Proof. intros ????. unfold sem_ty_ref; by repeat f_equiv. Qed.
+
+  Global Instance sem_ty_ref_cpy_proper : Proper ((≡) ==> (≡)) (@sem_ty_ref_cpy Σ _).
+  Proof. intros ????. unfold sem_ty_ref_cpy; by repeat f_equiv. Qed.
 
   Global Instance sem_ty_forall_proper ρ:
     Proper (pointwise_relation _ (≡) ==> (≡)) (sem_ty_forall ρ).
@@ -379,7 +484,7 @@ Section types_properties.
     Proper (pointwise_relation _ (≡) ==>(≡)) sem_ty_exists.
   Proof. 
     intros ????. unfold sem_ty_exists; repeat f_equiv.
-    by apply sem_ty_equiv.
+    by apply non_dep_fun_equiv.
   Qed.
 
   Global Instance sem_ty_rec_proper :
