theories/case_studies/asynchronous.v
@@ -1,0 +1,98 @@
+
+From stdpp Require Import base list.
+From iris.proofmode Require Import base tactics.
+From iris.algebra Require Import excl_auth.
+
+
+(* Hazel Reasoning *)
+From program_logic Require Import weakest_precondition 
+                                  tactics 
+                                  shallow_handler_reasoning 
+                                  deep_handler_reasoning 
+                                  state_reasoning.
+
+(* Local imports *)
+From affine_tes.lib Require Import base.
+From affine_tes.lang Require Import hazel.
+From affine_tes.logic Require Import sem_def.
+From affine_tes.logic Require Import sem_env.
+From affine_tes.logic Require Import sem_types.
+From affine_tes.logic Require Import reasoning.
+From affine_tes.logic Require Import sem_sub_typing.
+From affine_tes.logic Require Import sem_operators.
+From affine_tes.logic Require Import compatibility.
+From affine_tes.logic Require Import tactics.
+
+Definition async : val := (λ: "c", perform: (InjL "c"))%V.
+Definition await : val := (λ: "p", (perform: (InjR "p")) ;; #())%V.
+Definition yield : val := (λ: <>, await (async (λ: <>, #())))%V.
+
+Definition async' : val := 
+    (λ: "c", let: "r" := ref NONE
+             in (async (λ: <>, "r" <- SOME ("c" #())), "r"))%V.  
+                                    
+Section typing.
+
+  Context `{!heapGS Σ}.
+
+  Definition queue_ty := (μT: α, Ref (List (α → α))).
+
+  Definition prom_id := (@sem_ty_unit Σ).
+
+  Definition status_ty := (() + (List (queue_ty → queue_ty))).
+
+  Definition promise_ty := (Ref status_ty).
+
+  Definition cpromise_ty τ := (prom_id × Ref (Option τ)). 
+
+  Definition asig := (μS: α, ( () -{ α }-∘ () ) + prom_id ⇒ prom_id)%R. 
+
+  Lemma async_typed :
+    ⊢ ⊨ᵥ async : ( (() -{ asig }-∘ ()) -{ asig }-> prom_id ).
+  Proof.
+    iIntros "". iApply sem_typed_closure.
+    iApply (sem_typed_perform with "[]").
+    { intros ????. by repeat f_equiv. } 
+    iApply sem_typed_left_inj.
+    iApply sem_typed_sub_nil.
+    iApply sem_typed_var.
+  Qed.
+
+  Lemma await_typed :
+    ⊢ ⊨ᵥ await : ( prom_id -{ asig }-> () ).
+  Proof.
+    iIntros "". iApply sem_typed_closure.
+    iApply sem_typed_seq.
+    - iApply (sem_typed_perform with "[]").
+      { intros ????. by repeat f_equiv. } 
+      iApply sem_typed_sub_nil.
+      iApply sem_typed_right_inj.
+      iApply sem_typed_var. 
+    - iApply sem_typed_sub_nil.
+      iApply sem_typed_unit.
+  Qed.
+
+  Lemma yield_typed :
+    ⊢ ⊨ᵥ yield : ( () -{ asig }-> () ).
+  Proof.
+    iIntros "". iApply sem_typed_closure. simpl.
+    rewrite [Val await](@app_mult_env_dom_nil Σ) - {3} (app_nil_r []).
+    iApply (sem_typed_app _ [] _ _ _ _ _ prom_id).
+    { iApply sem_typed_sub_nil.
+      iApply sem_typed_val.
+      iApply await_typed. }
+    rewrite [Val async](@app_mult_env_dom_nil Σ).
+    iApply (sem_typed_app _ [] _ _ _ _ _ _).
+    { iApply sem_typed_sub_nil.
+      iApply sem_typed_val.
+      iApply async_typed. }
+    iApply sem_typed_sub_nil.
+    rewrite [(λ: <>, _)%E](@ctx_lambda_env_dom_nil Σ).
+    rewrite -(app_nil_r []).
+    iApply (sem_typed_afun _ _ [] []); solve_sidecond. simpl.
+    iApply sem_typed_sub_nil.
+    iApply sem_typed_unit.
+  Qed.
+
+
+End typing.
