theories/logic/tactics.v
@@ -1,0 +1,66 @@
+
+From iris.proofmode Require Import base tactics.
+
+(* Hazel Reasoning *)
+From program_logic Require Import weakest_precondition 
+                                  tactics 
+                                  shallow_handler_reasoning 
+                                  deep_handler_reasoning 
+                                  state_reasoning.
+
+(* Local imports *)
+From affine_tes.lib Require Import base.
+From affine_tes.lib Require Import logic.
+From affine_tes.lang Require Import hazel.
+From affine_tes.lang Require Import subst_map.
+From affine_tes.logic Require Import iEff.
+From affine_tes.logic Require Import sem_def.
+From affine_tes.logic Require Import sem_types.
+From affine_tes.logic Require Import sem_env.
+
+
+Ltac ewp_bottom := iApply ewp_os_prot_mono; 
+                   [by iApply iEff_le_bottom|].
+
+Ltac solve_dom := 
+    try rewrite !env_dom_nil;
+    try rewrite !env_dom_cons; 
+    repeat (
+      (by apply not_elem_of_nil) ||
+      (by apply not_elem_of_cons; split; solve_dom) || 
+        (intros ?; match goal with
+          | H : (BAnon ∈ _) |- _ => destruct H
+          end) ||
+    done).
+  
+Ltac solve_disjoint := 
+    repeat (
+      apply disjoint_empty ||
+      apply disjoint_cons_inv ||
+      done
+    ).
+
+Global Ltac solve_copy :=
+  repeat (
+    rewrite !env_sem_typed_empty ||
+    rewrite !env_sem_typed_cons ||
+    intros ? ||
+    apply bi.emp_persistent ||
+    apply bi.sep_persistent ||
+    apply bi.and_persistent ||
+    apply bi.or_persistent ||
+    apply bi.forall_persistent ||
+    apply bi.exist_persistent ||
+    apply bi.pure_persistent ||
+    apply plainly_persistent ||
+    apply bi.later_persistent ||
+    apply bi.persistently_persistent ||
+    apply bi.intuitionistically_persistent ||
+    apply inv_persistent).
+
+  Ltac solve_sidecond := 
+      try rewrite !env_dom_nil;
+      try rewrite !env_dom_cons;
+      solve_dom; 
+      solve_disjoint;
+      solve_copy.
